\lecture{6}{18 Jan. 11:00}{Hahn-Kolmogorov Theorem and Extension.}
Let's continue the proof of \autoref{thm:Hahn-Kolmogorov-Thm}.
\begin{proof}[Proof of \autoref{thm:Hahn-Kolmogorov-Thm} (cont.)]\label{pf:Hahn-Kolmogorov-Thm-cont}
	We proved the first part already, now we prove the part left.
	\begin{claim}
		\(\at{\mu }{\mathcal{\MakeUppercase{a}} _0}{} = \mu _0\).
	\end{claim}
	\begin{explanation}
		Let \(A\in \mathcal{A} _0\), we want to show that
		\[
			\mu (A) = \mu_0(A).
		\]
		\begin{itemize}
			\item Firstly, let
			      \[
				      B_{i} = \begin{dcases}
					      A,            & \text{ if } i= 1    \\
					      \varnothing , & \text{ if } i\geq 2
				      \end{dcases}\in \mathcal{A} _0,
			      \]
			      hence \(\bigcup\limits_{i=1}^{\infty} B_{i} = A\), then we see that
			      \[
				      \mu ^{\ast} (A)\leq \sum\limits_{i=1}^{\infty} \mu _0(B_{i}) = \mu _0(A)
			      \]
			      from the \hyperref[prop:outer-measure]{definition} of \(\mu ^{\ast} \) and \hyperref[def:pre-measure-countable-additivity-within-the-algebra]{countable additivity within the algebra}
			      of \(\mu _0\).
			\item Secondly, let \(B_{i}\in \mathcal{A} _0\), \(\bigcup\limits_{i=1}^{\infty} B_{i}\supset A\) be arbitrary.
			      Let \(C_1 = A\cap B_1\in \mathcal{A} _0\), \(C_{i} = A\cap B_{i}\setminus \left(\bigcup\limits_{j=1}^{i-1} B_{j}\right)\in \mathcal{A} _0\) for \(i\geq 2\)
			      since the operations are finite. Then we see
			      \[
				      A = \bigcup\limits_{i=1}^{\infty} C_{i}\in \mathcal{A} _0
			      \]
			      are disjoint countable unions, by \hyperref[def:pre-measure-countable-additivity-within-the-algebra]{countable additivity within the algebra},
			      we therefore have
			      \[
				      \mu _0(A) = \sum\limits_{i=1}^{\infty} \mu _0(C_{i}) \leq \sum\limits_{i=1}^{\infty} \mu_0 (B_{i})\implies \mu _0(A)\leq \mu ^{\ast} (A)
			      \]
			      by taking the infimum from the \hyperref[prop:outer-measure]{definition} of \(\mu ^{\ast} \).
		\end{itemize}
		Combine these two inequality, we see that
		\[
			\mu ^{\ast} (A) = \mu _0(A),
		\]
		for every \(A\in\mathcal{A} _0\), which implies \(\mu (A) = \mu _0(A)\) for every \(A\in \mathcal{A}_0\) from \autoref{thm:Caratheodory-extension-Thm},
		where we extend \(\mu ^{\ast} \) to \(\mu \) respect to \(\mathcal{A}_0\).
	\end{explanation}
\end{proof}

\begin{definition}[Hahn-Kolmogorov extension]\label{def:HK-extension}
	\((\mathcal{A} , \mu )\) obtained from \autoref{thm:Hahn-Kolmogorov-Thm} is the \emph{Hahn-Kolmogorov extensions} of \((\mathcal{A} _0, \mu _0)\).
\end{definition}
\begin{note}
	We sometimes say \emph{HK extension} instead of \hyperref[def:HK-extension]{Hahn-Kolmogorov extensions} for simplicity.
\end{note}

We can show the uniqueness of \hyperref[def:HK-extension]{HK extension}.

\begin{theorem}[Uniqueness of HK extension]\label{thm:uniqueness-of-HK-extension}
	Let \(\mathcal{A}_0\) be an \hyperref[def:algebra]{algebra} on \(X\), \(\mu _0\) be a \hyperref[def:pre-measure]{pre-measure} on \(\mathcal{A} _0\). Let \((\mathcal{A} , \mu)\)
	be the \hyperref[def:HK-extension]{HK extension} of \((\mathcal{A} _0, \mu _0)\). Let \((\mathcal{A} ^\prime , \mu ^\prime )\) be another extension of \((\mathcal{A} _0, \mu _0)\).
	Then if \(\mu _0\) is \hyperref[def:sigma-finite-measure]{\(\sigma\)-finite}, \(\mu  = \mu ^\prime \) on \(\mathcal{A} \cap \mathcal{A} ^\prime \).
\end{theorem}
\begin{proof}
	First, we note the following.
	\begin{note}
		Notice that \(\mathcal{A}_0 \subset \mathcal{A}, \mathcal{A} ^\prime \) since they both extend \(\mathcal{A}_0\).
	\end{note}

	Let \(A\in \mathcal{A} \cap \mathcal{A} ^\prime \), we need to show
	\[
		\underbrace{\mu (A)}_{\mu ^{\ast} (A)} = \mu ^\prime (A).
	\]
	We'll show this by showing two inequalities. We first show that \(\mu ^{\ast} (A)\geq \mu ^\prime (A)\).

	\begin{claim}
		\(\mu ^{\ast} (A)\geq \mu ^\prime (A)\).
	\end{claim}
	\begin{explanation}
		It's easy to show that \(\mu ^{\ast} (A)\geq \mu ^\prime (A)\) by choosing the arbitrary cover of \(A\) and using the \hyperref[prop:outer-measure]{definition}  of
		\(\mu ^{\ast} \).
	\end{explanation}

	Secondly, we will show that \(\mu (A)\leq \mu ^\prime (A)\).
	\begin{claim}
		\(\mu (A)\leq \mu ^\prime (A)\).
	\end{claim}
	\begin{explanation}
		We split this into two cases.
		\begin{itemize}
			\item \label{pf:uniqueness-of-HK-extension-2.i}Assume \(\mu (A)<\infty \), and fix \(\epsilon >0\). Then there exists \(B_{i}\in\mathcal{A} _0\) with \(B\coloneqq \bigcup\limits_{i=1}^{\infty} B_{i}\supset A\)
			      such that
			      \[
				      \mu (A)+\epsilon = \mu ^{\ast} (A) + \epsilon\overset{\hyperref[prop:outer-measure]{!}}{\geq} \sum\limits_{i=1}^{\infty} \mu _0(B_{i}) \overset{\hyperref[def:pre-measure-countable-additivity-within-the-algebra]{!}}{=} \sum\limits_{i=1}^{\infty} \mu (B_{i})\geq \mu \left(\bigcup\limits_{i=1}^{\infty} B_{i}\right) = \mu (B).
			      \]
			      This implies that
			      \[
				      \mu (B\setminus A) = \mu (B) - \mu (A)\leq \epsilon,
			      \]
			      where the equality comes from \(A\subset B\) and \(\mu (A)<\infty \). On the other hand,
			      \[
				      \mu (B) = \lim\limits_{N \to \infty} \mu \left(\bigcup\limits_{i=1}^{N} B_{i}\right) = \lim\limits_{N \to \infty} \mu ^\prime \left(\bigcup\limits_{i=1}^{N} B_{i}\right) = \mu ^\prime (B)
			      \]
			      where the middle equality follows from \(\mu  = \mu ^\prime \) on \(\mathcal{A} _0\), hence,
			      \[
				      \mu (A)\leq \mu (B) = \mu ^\prime (B) = \mu ^\prime (A)+\mu ^\prime (B\setminus A) \leq \mu ^\prime (A) + \mu (B\setminus A) \leq \mu ^\prime (A) + \epsilon
			      \]
			      for arbitrary \(\epsilon \), so we conclude \(\mu (A)\leq \mu ^\prime (A)\).
			\item Assume \(\mu (A) = \infty \). Since \(\mu _0\) is \hyperref[def:finite-measure]{\(\sigma \)-finite}, so we know \(X = \bigcup\limits_{n=1}^{\infty} X_{n}\) for some \(X_{n}\in\mathcal{A} _0\) such that
			      \(\mu _0(X_{n})<\infty\).  Replacing \(X_{n}\) by \(X_{1}\cup \ldots \cup X_{n} \in\mathcal{A} _0\), we may assume that \(X_1 \subset X_2 \subset \ldots\).
			      Then,
			      \[
				      \underset{n\in\mathbb{\MakeUppercase{N}} }{\forall}\ \mu (A \cap X_{n})<\infty\overset{\hyperref[pf:uniqueness-of-HK-extension-2.i]{!}}{\implies} \mu (A\cap X_{n})\leq \mu ^\prime (A\cap X_{n}).
			      \]

			      By \hyperref[thm:measure-space-continuity-from-above]{continuity from above}, we have
			      \[
				      \mu (A) = \lim\limits_{n \to \infty} \mu (A\cap X_{n})\leq \lim\limits_{n \to \infty} \mu ^\prime (A\cap X_{n}) = \mu ^\prime (A).
			      \]
		\end{itemize}
		Combine above two inequalities, the result follows.
	\end{explanation}
\end{proof}

\begin{corollary}\label{col:lec-6}
	Let \(\mu _0\) be a \hyperref[def:pre-measure]{pre-measure} on \hyperref[def:algebra]{algebra} \(\mathcal{A} _0\) on \(X\). Suppose \(\mu _0\) is
	\hyperref[def:finite-measure]{\(\sigma \)-finite}, then there exists a unique \hyperref[def:measure]{measure} \(\mu\) on \(\left< \mathcal{A} _0 \right> \)
	that extends \(\mathcal{A} _0\).

	Furthermore,
	\begin{enumerate}[(1)]
		\item The \hyperref[def:complete-measure-space]{completion} of \((X, \left< \mathcal{A} _0 \right>, \mu  )\) is the \hyperref[def:HK-extension]{HK extension} of
		      \((\mathcal{A} _0, \mu _0)\).\footnote{This really means the pair of the \hyperref[def:sigma-algebra]{\(\sigma\)-algebra} and the \hyperref[def:measure]{measure} in
			      the \hyperref[def:complete]{completion} of \((X, \left< \mathcal{\MakeUppercase{a}} _0 \right>, \mu  )\) is the \hyperref[def:HK-extension]{HK extension} of \((\mathcal{A} _0, \mu _0)\),
			      not the whole tuple of the \hyperref[def:measurable-space]{measurable-space}.}
		\item \(\mu (A) = \inf\left\{\sum\limits_{i=1}^{\infty} \mu _0(B_{i})\mid \underset{i\in\mathbb{\MakeUppercase{N}} }{\forall}\ B_{i}\in \mathcal{A} _0, \bigcup\limits_{i=1}^{\infty} B_{i}\supset A\right\}\)
		      for all \(A\in \overline{\left< \mathcal{A} _0 \right> }\).
	\end{enumerate}
\end{corollary}