\lecture{24}{09 Mar. 10:00}{Chain Homotopy}
To prove \autoref{thm:functoriality-is-homotopy-invariant}, we introduce some \hyperref[sec:homological-algebra]{homological algebra}.

\begin{definition}[Chain homotopy]\label{def:chain-homotopy}
	Given \hyperref[def:chain-complex]{chain complexes} \((A_\ast, \partial ^A_\ast)\) and \((B_\ast, \partial^B_\ast)\)
	and \hyperref[def:chain-map]{chain maps} \(f_\#, g_\# \colon  A_\ast \to B_\ast\). A \emph{chain homotopy} from
	\(f_\#\) to \(g_\#\) is a sequence of group homomorphisms \(\psi_n\colon A_n \to B_{n + 1}\) such that
	\[
		f_n - g_n = \partial ^B_{n + 1} \circ \psi_n + \psi_{n - 1} \circ \partial _n^A.
	\]
	In diagram, letting \(h_n \coloneqq f_n - g_n\), we have the following.
	\[
		\begin{tikzcd}
			\ldots && {A_{n+1}} && {A_{n}} && {A_{n-1}} && \ldots \\
			\\
			\ldots && {B_{n+1}} && {B_{n}} && {B_{n-1}} && \ldots
			\arrow["{\partial^A_{n-1}}", from=1-7, to=1-9]
			\arrow["{\partial^B_{n-1}}", from=3-7, to=3-9]
			\arrow["{\partial^A_{n}}", color={rgb,255:red,92;green,92;blue,214}, from=1-5, to=1-7]
			\arrow["{\partial^B_{n}}", from=3-5, to=3-7]
			\arrow["{\partial^B_{n+1}}", color={rgb,255:red,92;green,92;blue,214}, from=3-3, to=3-5]
			\arrow["{\partial^A_{n+2}}", from=1-1, to=1-3]
			\arrow["{\partial^B_{n+2}}", from=3-1, to=3-3]
			\arrow["{h_{n+1}}", from=1-3, to=3-3]
			\arrow["{h_{n}}", color={rgb,255:red,214;green,92;blue,92}, from=1-5, to=3-5]
			\arrow["{h_{n-1}}", from=1-7, to=3-7]
			\arrow["{\partial^A_{n+1}}", from=1-3, to=1-5]
			\arrow["{\psi_n}"', color={rgb,255:red,92;green,92;blue,214}, from=1-5, to=3-3]
			\arrow["{\psi_{n-1}}"', color={rgb,255:red,92;green,92;blue,214}, from=1-7, to=3-5]
		\end{tikzcd}
	\]
	This diagram does \textbf{not} commute, however, the \textbf{\textcolor{red}{red}} map is the sum of the
	\textbf{\textcolor{blue}{blue}} maps composed up, so it shows everything that is going on.
\end{definition}

\begin{theorem}\label{thm:chain-homotopies-on-homology}
	If there is a \hyperref[def:chain-homotopy]{chain homotopy} \(\psi\) from \(f_\#\) to \(g_\#\), then the induced maps
	\(f_\ast, g_\ast\) on \hyperref[def:homology-group]{homology} are equal.
\end{theorem}
\begin{proof}
	Let \(\sigma \in A_n\) be an \(n\)-cycle, i.e. \(\partial_n^A \sigma = 0\). Then we compute that:
	\[
		(f_n - g_n)(\sigma) = \partial_{n + 1}^B(\psi_n(\sigma)) + \psi_{n - 1}(\partial_n^A(\sigma)) = \partial_{n + 1}^B(\psi_n(\sigma)) \in \im (\partial^B_{n + 1}).
	\]

	This tells us that \((f_n - g_n)(\sigma)\) is a \hyperref[def:boundary]{boundary}, and so \((f_n - g_n)(\sigma) = 0\) when considered as an element of
	the \hyperref[def:homology-group]{homology group} (with degree \(n\)).
	Thus, \(f_n(\sigma) = g_n(\sigma)\) in the \hyperref[def:homology-group]{homology group}, and so \(f, g\) induce the same map as desired.
\end{proof}

We now sketch the proof of \autoref{thm:functoriality-is-homotopy-invariant} given in Hatcher\cite{hatcher2002algebraic}. From this point in the course many
of the theorems require much more algebraic work than we are interested in. We instead want to learn how to use the computational tools.
\begin{proof}[Proof sketch of \autoref{thm:functoriality-is-homotopy-invariant}]\label{pf:functoriality-is-homotopy-invariant}
	Suppose we have some \hyperref[def:homotopy]{homotopy} \(F \colon I \times X \to Y\) from \(f\) to \(g\). The most difficulty
	in this proof is the combinatorial difficulty involved in the fact that the product of a \hyperref[def:standard-simplex]{simplex}
	in \(X\) and \(I\) is not a \hyperref[def:standard-simplex]{simplex}.

	We now consider
	\begin{enumerate}[(1)]
		\item Subdivide \(\Delta^n \times I\) into \((n + 1)\)-dimensional \hyperref[def:subsimplex]{subsimplices}.\footnote{We want to do this since the
			      product between two \hyperref[def:standard-simplex]{simplices} is not a \hyperref[def:standard-simplex]{simplex}, as we just note.}
		      \begin{figure}[H]
			      \centering
			      \incfig{pf:functoriality-is-homotopy-invariant}
			      \label{fig:pf:functoriality-is-homotopy-invariant}
		      \end{figure}
		\item We define the \underline{prism} operator:
		      \[
			      \begin{split}
				      P_n \colon C_n(X)         & \to C_{n + 1}(Y)\\
				      [\sigma \colon \Delta^n \to X] & \mapsto \begin{bmatrix} \text{ alternating sums of restrictions }                                             \\
					      \Delta^n \times I \xrightarrow{\sigma \times \identity } X \times I \xrightarrow{F} Y \\
					      \text{ to each \hyperref[def:standard-simplex]{simplex} in our subdivision }
				      \end{bmatrix}
			      \end{split}
		      \]
		\item We now need to check that
		      \[
			      \partial_{n + 1}^YP_n = \fcolorbox{blue}{white}{\(g_\#\)} - \fcolorbox{red}{white}{\(f_\#\)} - \fcolorbox{green}{white}{\(P_{n - 1}\partial_n^X\)}.
		      \]

		      We have the following diagram.
		      \begin{figure}[H]
			      \centering
			      \incfig{pf:functoriality-is-homotopy-invariant-2}
			      \label{fig:pf:functoriality-is-homotopy-invariant-2}
		      \end{figure}
		      Thus \(P\) is a \hyperref[def:chain-homotopy]{chain homotopy}, and we're done.
	\end{enumerate}
\end{proof}